Add sequence flattening to polyloop

PolyLoop.v
@@ -26,6 +26,7 @@ Inductive poly_stmt :=
 | PSkip : poly_stmt
 | PSeq : poly_stmt -> poly_stmt -> poly_stmt
 | PGuard : polyhedron -> poly_stmt -> poly_stmt.
+(* | PStrideGuard : list affine_expr -> poly_stmt -> poly_stmt. *)
 
 Inductive poly_loop_semantics : poly_stmt -> list Z -> mem -> mem -> Prop :=
 | PLInstr : forall i es env mem1 mem2,
@@ -85,6 +86,12 @@ Proof.
   inversion_clear H. exists mem2; auto.
 Qed.
 
+Lemma PLSkip_inv_sem :
+  forall env mem1 mem2, poly_loop_semantics PSkip env mem1 mem2 -> mem1 = mem2.
+Proof.
+  intros env mem1 mem2 H; inversion H; congruence.
+Qed.
+
 Fixpoint make_seq l :=
   match l with
   | nil => PSkip
@@ -98,4 +105,41 @@ Proof.
   induction l.
   - intros; split; intros H; inversion_clear H; constructor.
   - intros; split; simpl; intros H; inversion_clear H; econstructor; eauto; rewrite IHl in *; eauto.
+Qed.
+
+Fixpoint flatten_seq_rec stmt atend :=
+  match stmt with
+  | PSeq st1 st2 => flatten_seq_rec st1 (flatten_seq_rec st2 atend)
+  | PSkip => atend
+  | stmt => PSeq stmt atend
+  end.
+
+Lemma flatten_seq_rec_semantics :
+  forall s atend env mem1 mem2, poly_loop_semantics (flatten_seq_rec s atend) env mem1 mem2 <-> poly_loop_semantics (PSeq s atend) env mem1 mem2.
+Proof.
+  induction s; intros atend env mem1 mem2; simpl in *; try reflexivity.
+  - split.
+    + intros H; econstructor; [constructor|auto].
+    + intros H; apply PLSeq_inv_sem in H; destruct H as [mem3 [H1 H2]]; apply PLSkip_inv_sem in H1; congruence.
+  - rewrite IHs1. split.
+    + intros H.
+      apply PLSeq_inv_sem in H; destruct H as [mem3 [H1 H2]]; rewrite IHs2 in H2.
+      apply PLSeq_inv_sem in H2; destruct H2 as [mem4 [H2 H3]]. 
+      econstructor; [econstructor|]; eauto.
+    + intros H.
+      apply PLSeq_inv_sem in H; destruct H as [mem3 [H1 H2]].
+      apply PLSeq_inv_sem in H1; destruct H1 as [mem4 [H1 H3]].
+      econstructor; [eauto|].
+      rewrite IHs2; econstructor; eauto.
+Qed.
+
+Definition flatten_seq stmt := flatten_seq_rec stmt PSkip.
+
+Lemma flatten_seq_semantics :
+  forall s env mem1 mem2, poly_loop_semantics (flatten_seq s) env mem1 mem2 <-> poly_loop_semantics s env mem1 mem2.
+Proof.
+  intros s env mem1 mem2; unfold flatten_seq; rewrite flatten_seq_rec_semantics.
+  split.
+  - intros H; apply PLSeq_inv_sem in H; destruct H as [mem3 [H1 H2]]; apply PLSkip_inv_sem in H2. congruence.
+  - intros H; econstructor; [|constructor]; eauto.
 Qed.
